repackaging and refactoring

misc/while_props/WhileNoSuccess.ec
@@ -2,6 +2,247 @@ pragma Goals:printall.
 require import AllCore Distr.
 
 
+theory IterUntilSuccDistr.
+
+type sbits, iat, rrt, irt.
+
+module M = {
+  var c : int
+  proc whp(MyP : rrt -> bool,myd : rrt distr, s : int, e : int, r : rrt) = {
+    c <- s;
+    while(c <= e /\ !MyP r){
+     r <$ myd;
+     c <- c + 1;
+    }
+    return r;
+  }
+
+  proc whp_if_end(MyP : rrt -> bool,myd : rrt distr, s : int, e : int, r : rrt) = {
+    var ri : rrt;
+    ri <@ whp(MyP,myd, s,e,r);
+    if(c <= e + 1 /\ !MyP ri){
+      ri <$ myd;
+      c <- c + 1;
+    }
+    return ri;
+  }
+}.
+
+
+lemma whp_split_if_end :  
+  equiv[ M.whp ~ M.whp_if_end : ={MyP,myd, s,r} /\ e{1} - 1 = e{2}
+        ==> ={res,M.c} ].
+proof. proc.
+inline*. sp. 
+splitwhile{1} 1 : M.c  <= (e - 1) .
+seq  1 1 : (={M.c} /\ r{1} = r0{2} /\ myd{1} = myd0{2} /\ e0{2} = e{2} /\ myd0{2} = myd{2}
+   /\ MyP0{2} = MyP{1} /\ MyP0{2} = MyP{2} 
+   /\ e{1} - 1 = e0{2} /\ (!MyP{1} r{1} => (e{1} - 1) < M.c{1} )).
+while (={M.c,myd,MyP} /\ r{1} = r0{2} /\ myd{1} = myd0{2} /\ e0{2} = e{2} 
+   /\ MyP{1} = MyP0{2} /\ MyP{2} = MyP0{2}
+   /\ e{1} - 1 = e0{2} ).
+wp. rnd. skip.  progress. smt().  skip. progress. smt(). smt().
+sp. simplify.
+case (MyP{1} r{1}).
+rcondf {1} 1. progress. skip. smt().
+rcondf {2} 1. progress. skip. progress. smt().
+skip. progress.
+unroll {1} 1.
+if. progress.  
+rcondf {1} 3. progress.
+wp. rnd. skip. progress. smt().
+wp. rnd. skip. progress. 
+rcondf {1} 1. progress. skip. progress.
+qed.
+
+
+lemma whp_split_if_end' MyP s e r p P d :  
+  (phoare [ M.whp_if_end : arg = (MyP,d,s,e,r) ==> P res ] = p)
+   => phoare [ M.whp : arg = (MyP,d,s,e+1,r) ==> P res ] = p.
+proof. progress. bypr.
+progress.
+have <-: Pr[M.whp_if_end(MyP{m},d{m}, s{m}, e{m}, r{m}) @ &m : P res] = p.
+byphoare (_: arg = (MyP{m},d{m}, s{m}, e{m}, r{m}) ==> _).
+conseq H. auto. auto. byequiv.
+conseq whp_split_if_end. smt(). auto. auto. auto.
+qed.
+
+
+lemma lll (b a c : real) : a <= b => b <= c => a <= c.
+smt(). qed.
+
+    
+lemma whp_split_if_end_le MyP s e r p myd P :  
+  (phoare [ M.whp_if_end : arg = (MyP,myd,s,e,r) ==> P res ] <= p)
+   => phoare [ M.whp : arg = (MyP,myd,s,e+1,r) ==> P res ] <= p.
+proof. progress. bypr.
+progress.
+have zz : Pr[M.whp_if_end(MyP{m}, myd{m},s{m}, e{m}, r{m}) @ &m : P res] <= p.
+byphoare (_: arg = (MyP{m},myd{m},s{m}, e{m}, r{m}) ==> _).
+conseq H. auto. auto. 
+apply (lll Pr[M.whp_if_end(MyP,myd,s, e, r) @ &m : P res] ).
+byequiv.
+ conseq whp_split_if_end. smt(). auto. auto. auto. apply zz.
+qed.
+
+
+lemma whp_split_if_end_ge MyP s e r p myd P :  
+  (phoare [ M.whp_if_end : arg = (MyP,myd,s,e,r) ==> P res ] >= p)
+   => phoare [ M.whp : arg = (MyP,myd,s,e+1,r) ==> P res ] >= p.
+proof. progress. bypr.
+progress.
+have zz : Pr[M.whp_if_end(MyP{m}, myd{m},s{m}, e{m}, r{m}) @ &m : P res] >= p.
+byphoare (_: arg = (MyP{m},myd{m},s{m}, e{m}, r{m}) ==> _).
+conseq H. auto. auto.  
+apply (lll Pr[M.whp_if_end(MyP,myd,s, e, r) @ &m : P res] ). auto.
+byequiv. 
+symmetry. conseq whp_split_if_end. smt(). auto. auto. auto. 
+qed.
+
+
+
+lemma asdsad (p : real) r myda MyPa: 
+  (mu myda (fun (x : rrt) => ! MyPa x) = p) =>
+  MyPa r = false => forall e, 0 <= e => 
+  phoare[ M.whp_if_end : arg = (MyPa,myda, 1,e,r) ==> !MyPa res ] = (p ^ (e+1)).
+proof. move => iipr ipr. apply ge0ind. smt().
+progress. simplify.
+  progress. proc.
+inline*. sp.
+rcondf 1. skip. smt().
+sp. 
+rcondt 1. skip. progress. smt().
+swap 1 1.  rnd.  simplify.
+wp.  skip.  progress. smt(@Real).
+progress. proc.
+  have phf: phoare[ M.whp : arg = (MyPa,myda, 1, n+1, r) ==> !MyPa res] = (p ^(n+1)).
+ apply (whp_split_if_end'  MyPa 1 n r  (p^(n+1)) (fun x => !MyPa x) myda (H0 H) ).
+seq 1 : (!MyPa ri) (p ^(n+1)) p 1%r 0%r (myd = myda /\ MyP = MyPa /\ (!MyPa ri => M.c <= e + 1)).
+inline*. sp.
+seq 1 :  (MyP = MyPa /\ myd = myda  /\ (!MyPa r0 => M.c <= e + 1)).
+ while (MyP = MyP0 /\ MyP = MyPa /\ myd = myda /\ e = e0 /\ (!MyPa r0 => M.c <= e0 + 1)).
+wp. 
+rnd.  skip. progress. smt(). skip. progress. smt(). sp.  skip. progress. 
+ call phf. skip.  auto.
+rcondt 1. skip. progress. smt().  
+wp. simplify.  rnd.  simplify.
+skip. progress. 
+hoare. 
+rcondf 1. skip. progress. smt().
+simplify. skip. auto. progress. smt(@Real).
+qed.
+
+
+lemma asdsad_le (p : real) MyPa r d:
+  (mu d (fun (x : rrt) => ! MyPa x) <= p) =>
+    MyPa r = false => forall e, 0 <= e => 
+  phoare[ M.whp_if_end : arg = (MyPa, d,1,e,r) ==> !MyPa res ]
+     <= (p ^ (e+1)).
+proof. move => dpr ipr. apply ge0ind. smt().
+progress. simplify.
+  progress. proc.
+inline*. sp.
+rcondf 1. skip. smt().
+sp. 
+rcondt 1. skip. progress. smt().
+swap 1 1.  rnd.  simplify.
+wp.  skip.  progress. smt(@Real). 
+progress. proc.
+  have phf: phoare[ M.whp : arg = (MyPa,d,1, n+1, r) ==> !MyPa res] <= (p ^(n+1)).
+ apply (whp_split_if_end_le MyPa 1 n r (p^(n+1)) d (fun x => !MyPa x) (H0 H) ).
+seq 1 : (!MyP ri) (p ^(n+1)) p 1%r 0%r (d = myd /\ MyP = MyPa /\ (!MyP ri => M.c <= e + 1)).
+inline*. sp.
+seq 1 :  (d = myd /\ MyP = MyPa /\ myd = myd0 /\ (!MyP r0 => M.c <= e + 1)).
+ while (d = myd /\ myd = myd0 /\ MyP = MyP0 /\ e = e0 /\ (!MyP r0 => M.c <= e0 + 1)).
+wp. 
+rnd.  skip. progress. smt(). skip. progress. smt(). sp.  skip. progress. 
+ call phf. skip.  auto.
+rcondt 1. skip. progress. smt(). 
+wp. simplify.  rnd.  simplify.
+skip. progress.
+hoare. 
+rcondf 1. skip.  progress. smt().
+simplify. skip. auto. smt(@Real).
+qed.
+
+
+
+
+lemma asdsad_ge (p : real) MyPa r d:
+  (mu d (fun (x : rrt) => ! MyPa x) >= p) =>
+    MyPa r = false => forall e, 0 <= e => 
+  phoare[ M.whp_if_end : arg = (MyPa, d,1,e,r) ==> !MyPa res ]
+     >= (p ^ (e+1)).
+proof. move => dpr ipr. apply ge0ind. smt().
+progress. simplify.
+  progress. proc.
+inline*. sp.
+rcondf 1. skip. smt().
+sp. 
+rcondt 1. skip. progress. smt().
+swap 1 1.  rnd.  simplify.
+wp.  skip.  progress. smt(@Real). 
+progress. proc.
+  have phf: phoare[ M.whp : arg = (MyPa,d,1, n+1, r) ==> !MyPa res] >= (p ^(n+1)).
+ apply (whp_split_if_end_ge MyPa 1 n r (p^(n+1)) d (fun x => !MyPa x) (H0 H) ).
+seq 1 : (!MyP ri) (p ^(n+1)) p 1%r 0%r (d = myd /\ MyP = MyPa /\ (!MyP ri => M.c <= e + 1)).
+inline*. sp.
+seq 1 :  (d = myd /\ MyP = MyPa /\ myd = myd0 /\ (!MyP r0 => M.c <= e + 1)).
+ while (d = myd /\ myd = myd0 /\ MyP = MyP0 /\ e = e0 /\ (!MyP r0 => M.c <= e0 + 1)).
+wp. 
+rnd.  skip. progress. smt(). skip. progress. smt(). sp.  skip. progress. 
+ call phf. skip.  auto.
+rcondt 1. skip. progress. smt(). 
+wp. simplify.  rnd.  simplify.
+skip. progress.
+hoare. 
+rcondf 1. skip.  progress. smt().
+simplify. skip. auto. smt(@Real).
+qed.
+
+
+lemma asdsadq (p : real) MyP r d:  
+   (mu d (fun (x : rrt) => ! MyP x) = p) =>
+  MyP r = false => forall e, 0 <= e =>
+  phoare[ M.whp : arg = (MyP,d,1,e+1,r) ==> !MyP res ] = (p ^ (e+1)).
+move => H1 H e ep.
+have fact1  : phoare[ M.whp_if_end : arg = (MyP,d,1,e,r) ==> !MyP res ] = (p ^ (e+1)).
+apply (asdsad  p r d MyP H1 H e ep). auto.
+conseq (whp_split_if_end' MyP 1 e r (p^(e+1)) (fun x => !MyP x) d fact1).
+qed.
+
+
+
+lemma asdsadq_le (p : real) MyP r d:  
+   (mu d (fun (x : rrt) => ! MyP x) <= p) =>
+   MyP r = false => forall e, 0 <= e =>
+    phoare[ M.whp : arg = (MyP,d,1,e+1,r) ==> !MyP res ] <= (p ^ (e+1)).
+move => H1 H e ep.
+have fact1  : phoare[ M.whp_if_end : arg = (MyP,d,1,e,r) ==> !MyP res ] <= (p ^ (e+1)).
+apply (asdsad_le  p MyP r d H1 H e ep). auto.
+conseq (whp_split_if_end_le MyP 1 e r (p^(e+1))  d (fun x => !MyP x) fact1).
+qed.
+
+
+
+lemma asdsadq_ge (p : real) MyP r d:  
+   (mu d (fun (x : rrt) => ! MyP x) >= p) =>
+   MyP r = false => forall e, 0 <= e =>
+    phoare[ M.whp : arg = (MyP,d,1,e+1,r) ==> !MyP res ] >= (p ^ (e+1)).
+move => H1 H e ep.
+have fact1  : phoare[ M.whp_if_end : arg = (MyP,d,1,e,r) ==> !MyP res ] >= (p ^ (e+1)).
+apply (asdsad_ge  p MyP r d H1 H e ep). auto.
+conseq (whp_split_if_end_ge MyP 1 e r (p^(e+1))  d (fun x => !MyP x) fact1).
+qed.
+
+end IterUntilSuccDistr.
+
+
+
+
+
+theory IterIfNoSucc.
+
 type sbits, iat, rrt, irt.
 
 op pair_sbits : sbits * sbits -> sbits.
@@ -9,11 +250,53 @@ op unpair: sbits -> sbits * sbits.
 axiom ips: injective pair_sbits. 
 axiom unpair_pair x : unpair (pair_sbits x) = x.
 
-require WhileSplit.
-clone import WhileSplit as IM with type sbits <- sbits,
-                                   type iat <- iat,
-                                   type rrt <- rrt,
-                                   type irt <- irt.
+
+module type HasRun = {
+  proc run(z : irt) : rrt {}
+}.
+
+
+module W(A : HasRun) = {
+  var c : int
+  proc whp(p : rrt -> bool, i : irt, s : int, e : int, r : rrt) = {
+    c <- s;
+    while(c <= e /\ !p r){
+     r <@ A.run(i);
+     c <- c + 1;
+    }
+    return r;
+  }
+
+
+  proc if_whp(p : rrt -> bool, i : irt, s : int, e : int, r : rrt) = {
+    c <- s;
+    if(c <= e /\ !p r){
+     r <@ A.run(i);
+     c <- c + 1;
+    }
+    r <@ whp(p,i,W.c,e,r);
+    return r;
+  }
+
+  proc whp_if(p : rrt -> bool, i : irt, s : int, e : int, r : rrt) = {
+    var ri;
+    c <- s;
+    ri <@ whp(p,i,s,e-1,r);
+    if(c <= e /\ !p ri){
+     ri <@ A.run(i);
+     c <- c + 1;
+    }
+    return ri;
+  }
+
+  proc whp_split(p : rrt -> bool, i : irt, s : int, m : int, e : int, r : rrt) = {
+    c <- s;
+    r <@ whp(p,i,s,m,r);
+    r <@ whp(p,i,W.c,e,r);
+    return r;
+  }
+  
+}.
 
 
 
@@ -50,6 +333,11 @@ module DW = {
   }
 }.
 
+local clone import IterUntilSuccDistr with type sbits <- sbits,
+                                           type iat <- iat,
+                                           type rrt <- rrt,
+                                           type irt <- irt.
+  
 
 
 op MyPred : rrt -> bool.
@@ -61,7 +349,7 @@ declare axiom A_rew_ph x : phoare[ A.run : (glob A) = x ==> !MyPred res => (glob
 
 
 
-lemma A_rew_h x : hoare[ A.run : (glob A) = x ==> !MyPred res => (glob A) = x ] .
+local lemma A_rew_h x : hoare[ A.run : (glob A) = x ==> !MyPred res => (glob A) = x ] .
 bypr. progress. 
 have <- : Pr[A.run(z{m}) @ &m : false ] = 0%r. rewrite Pr[mu_false]. auto.
 have : 1%r = Pr[A.run(z{m}) @ &m : !(!MyPred res => (glob A) = (glob A){m}) ]
@@ -75,7 +363,7 @@ qed.
 
 
 
-lemma asdistr_rew2 : forall (D : (glob A) -> irt -> rrt distr) ,
+local lemma asdistr_rew2 : forall (D : (glob A) -> irt -> rrt distr) ,
   (forall &m M a, mu (D (glob A){m} a) M = Pr[ A.run(a) @ &m :  M res ])
   => forall &m a, equiv [SF.sampleFrom ~ A.run : ={glob A} /\ arg{1} = (D (glob A){m} a) 
                          /\ (glob A){2} = (glob A){m} /\ arg{2} = a 
@@ -135,10 +423,8 @@ rewrite hpp.
 qed.
 
 
-
-
   
-lemma zz  (da : (glob A) -> irt -> rrt distr) :  
+local lemma zz  (da : (glob A) -> irt -> rrt distr) :  
  (forall &m (M : rrt -> bool) (a : irt),
        mu (da (glob A){m} a) M = Pr[A.run(a) @ &m : M res])
  => forall &m P e (s : int) rr ia,  
@@ -203,7 +489,7 @@ progress.
 byphoare (_: e = 0 /\ s = 1 /\ p ra = false /\ r = ra ==> _).
 simplify. proc.
 sp.
-rcondf 1. skip. progress. skip. smt(@Real). smt(). auto.  auto. 
+rcondf 1. skip. progress. skip. smt(@Real). smt(). auto.  auto.
 move => ez sf ep.
 have :  exists e', e' + 1 = e /\ 0 <= e'. smt().
 elim. progress.
@@ -211,14 +497,14 @@ have exD :  exists (D : (glob A) -> irt -> rrt distr),
       forall &m (M : rrt -> bool) (a : irt),
         mu (D (glob A){m} a) M = Pr[A.run(a) @ &m : M res].
 apply (reflection_simple_res A).
-elim exD. progress. 
+elim exD. progress.
 rewrite - (zz  D H1 &m (fun x => !MyPred x)).
 have ->: Pr[DW.whp_d(MyPred,D (glob A){m} i, 1, e' + 1 , ra) @ &m : !MyPred res]
  = Pr[M.whp(MyPred,D (glob A){m} i, 1, e' + 1 , ra) @ &m : !MyPred res].
-byequiv. proc.  sp. 
+byequiv. proc.  sp.
 conseq (_: ={e,r} /\ p{1} = MyP{2} /\ DW.c{1} = M.c{2} /\ d{1} = myd{2}  ==> _). auto.
-while (={e,r} /\ p{1} = MyP{2} /\ DW.c{1} = M.c{2} /\ d{1} = myd{2}). wp. inline*. wp.  rnd. wp. 
-skip. progress. 
+while (={e,r} /\ p{1} = MyP{2} /\ DW.c{1} = M.c{2} /\ d{1} = myd{2}). wp. inline*. wp.  rnd. wp.
+skip. progress.
 skip. progress. auto. auto.
 byphoare(_: arg = (MyPred,D (glob A){m} i, 1, e' + 1 , ra ) ==> _).
 have lf :   mu (D (glob A){m} i) (fun (x : rrt) => ! MyPred x) <= pr. rewrite H1. auto.
@@ -229,16 +515,61 @@ qed.
 
 
 
+lemma final_zz_ge &m pr  i e ra :  MyPred ra = false => 0 <= e =>
+   Pr[ A.run(i) @ &m : !MyPred res ]  >= pr
+  => Pr[ W(A).whp(MyPred,i, 1,e,ra) @ &m : !MyPred res ] >= (pr ^ (e)).
+case (e = 0).
+progress.
+byphoare (_: e = 0 /\ s = 1 /\ p ra = false /\ r = ra ==> _).
+simplify. proc.
+sp.
+rcondf 1. skip. progress. skip. smt(@Real). smt(). auto.  auto.
+move => ez sf ep.
+have :  exists e', e' + 1 = e /\ 0 <= e'. smt().
+elim. progress.
+have exD :  exists (D : (glob A) -> irt -> rrt distr),
+      forall &m (M : rrt -> bool) (a : irt),
+        mu (D (glob A){m} a) M = Pr[A.run(a) @ &m : M res].
+apply (reflection_simple_res A).
+elim exD. progress.
+rewrite - (zz  D H1 &m (fun x => !MyPred x)).
+have ->: Pr[DW.whp_d(MyPred,D (glob A){m} i, 1, e' + 1 , ra) @ &m : !MyPred res]
+ = Pr[M.whp(MyPred,D (glob A){m} i, 1, e' + 1 , ra) @ &m : !MyPred res].
+byequiv. proc.  sp.
+conseq (_: ={e,r} /\ p{1} = MyP{2} /\ DW.c{1} = M.c{2} /\ d{1} = myd{2}  ==> _). auto.
+while (={e,r} /\ p{1} = MyP{2} /\ DW.c{1} = M.c{2} /\ d{1} = myd{2}). wp. inline*. wp.  rnd. wp.
+skip. progress.
+skip. progress. auto. auto.
+byphoare(_: arg = (MyPred,D (glob A){m} i, 1, e' + 1 , ra ) ==> _).
+have lf :   mu (D (glob A){m} i) (fun (x : rrt) => ! MyPred x) >= pr. rewrite H1. auto.
+conseq (asdsadq_ge pr MyPred ra (D (glob A){m} i) lf sf e' H ). auto.
+auto.
+qed.
+
+
 lemma final_zz_ph_le p  i e r :  MyPred r = false => 0 <= e =>
    phoare[ A.run : arg = i ==> !MyPred res ] <= p =>
    phoare [ W(A).whp : arg = (MyPred, i, 1,e,r) ==> !MyPred res ] <= (p ^ (e)).
 move => sf ep ph1.
 bypr. progress.
-have ff : Pr[A.run(i) @ &m : ! MyPred res] <= p. 
+have ff : Pr[A.run(i) @ &m : ! MyPred res] <= p.
 byphoare (_: arg = i ==> _). apply ph1. auto. auto.
 rewrite H. simplify.
 apply (final_zz_le &m p  i e r sf ep ff).
 qed.
+
+
+lemma final_zz_ph_ge p  i e r :  MyPred r = false => 0 <= e =>
+   phoare[ A.run : arg = i ==> !MyPred res ] >= p =>
+   phoare [ W(A).whp : arg = (MyPred, i, 1,e,r) ==> !MyPred res ] >= (p ^ (e)).
+move => sf ep ph1.
+bypr. progress.
+have ff : Pr[A.run(i) @ &m : ! MyPred res] >= p.
+byphoare (_: arg = i ==> _). apply ph1. auto. auto.
+rewrite H. simplify.
+apply (final_zz_ge &m p  i e r sf ep ff).
+qed.
+
 
 
 lemma final_zz_ph &m p i e r :  MyPred r = false => 0 <= e =>
@@ -258,10 +589,267 @@ lemma final_zz_ph_m &m p i e r :  MyPred r = false => 0 <= e =>
    phoare [ W(A).whp : arg = (MyPred,i, 1,e,r) /\ (glob A){m} = (glob A) ==> !MyPred res ] = (p ^ e).
 move => sf ep ph1.
 bypr. progress. rewrite H. simplify.
-rewrite -  (final_zz &m0 p  i e r sf ep). 
+rewrite -  (final_zz &m0 p  i e r sf ep).
 byphoare (_: arg = i /\ (glob A) = (glob A){m0} ==> _). conseq ph1. auto. auto.
 auto. auto.
 qed.
 
 
 end section.
+
+end IterIfNoSucc.
+
+
+theory IterUntilSucc.
+
+type rt, iat.
+
+module type Run = {
+  proc run(i:iat) : rt
+}.
+
+module M(A : Run) = {
+  var c : int
+  proc whp(i : iat, MyP : rt -> bool, s : int, e : int, r : rt) = {
+    c <- s;
+    while(c <= e /\ !MyP r){
+     r <@ A.run(i);
+     c <- c + 1;
+    }
+    return r;
+  }
+
+  proc whp_if_end(i : iat, MyP : rt -> bool,s : int, e : int, r : rt) = {
+    var ri : rt;
+    ri <@ whp(i,MyP, s,e,r);     
+    if(c <= e + 1 /\ !MyP ri){
+      ri <@ A.run(i);
+      c <- c + 1;
+    }
+    return ri;
+  }
+}.
+
+section.
+declare module A <: Run{-M}.
+
+declare axiom A_run_ll : islossless A.run.
+
+lemma whp_split_if_end :  
+  equiv[ M(A).whp ~ M(A).whp_if_end : ={glob A, i, MyP, s,r} /\ e{1} - 1 = e{2}
+        ==> ={res,M.c} ].
+proof. proc.
+inline*. sp. 
+splitwhile{1} 1 : M.c  <= (e - 1) .
+seq  1 1 : (={M.c, glob A} /\ r{1} = r0{2} /\ e0{2} = e{2} /\ i{1} = i0{2} /\ i{2} = i0{2}
+   /\ MyP0{2} = MyP{1} /\ MyP0{2} = MyP{2} 
+   /\ e{1} - 1 = e0{2} /\ (!MyP{1} r{1} => (e{1} - 1) < M.c{1} )).
+while (={M.c,MyP, glob A} /\ r{1} = r0{2} /\ e0{2} = e{2} /\ i{1} = i0{2} /\ i{2} = i0{2}
+   /\ MyP{1} = MyP0{2} /\ MyP{2} = MyP0{2}
+   /\ e{1} - 1 = e0{2} ).
+wp. call (_:true).   skip. progress. smt(). skip. progress. smt(). smt().
+sp. simplify.
+case (MyP{1} r{1}).
+rcondf {1} 1. progress. skip. smt().
+rcondf {2} 1. progress. skip. progress. smt().
+skip. progress.
+unroll {1} 1.
+if. progress.  
+rcondf {1} 3. progress.
+wp. call (_:true). skip. progress. smt().
+wp. call (_:true). skip. progress. 
+rcondf {1} 1. progress. skip. progress.
+qed.
+
+
+
+lemma whp_split_if_end' MyP  i s e r p P :  
+  (phoare [ M(A).whp_if_end : arg = (i,MyP,s,e,r) ==> P res ] = p)
+   => phoare [ M(A).whp : arg = (i, MyP,s,e+1,r) ==> P res ] = p.
+proof. progress. bypr.
+progress.
+have <-: Pr[M(A).whp_if_end(i{m}, MyP{m}, s{m}, e{m}, r{m}) @ &m : P res] = p.
+byphoare (_: arg = (i{m}, MyP{m}, s{m}, e{m}, r{m}) ==> _).
+conseq H. auto. auto. byequiv.
+conseq whp_split_if_end. smt(). auto. auto. auto.
+qed.
+
+
+lemma lll (b a c : real) : a <= b => b <= c => a <= c.
+smt(). qed.
+
+    
+lemma whp_split_if_end_le MyP i s e r p P :  
+  (phoare [ M(A).whp_if_end : arg = (i,MyP,s,e,r) ==> P res ] <= p)
+   => phoare [ M(A).whp : arg = (i,MyP,s,e+1,r) ==> P res ] <= p.
+proof. progress. bypr.
+progress.
+have zz : Pr[M(A).whp_if_end(i{m},MyP{m}, s{m}, e{m}, r{m}) @ &m : P res] <= p.
+byphoare (_: arg = (i{m},MyP{m},s{m}, e{m}, r{m}) ==> _).
+conseq H. auto. auto. 
+apply (lll Pr[M(A).whp_if_end(i, MyP,s, e, r) @ &m : P res] ).
+byequiv.
+conseq whp_split_if_end. smt(). auto. auto. auto. apply zz.
+qed.
+
+
+lemma whp_split_if_end_ge MyP i s e r p P :  
+  (phoare [ M(A).whp_if_end : arg = (i,MyP,s,e,r) ==> P res ] >= p)
+   => phoare [ M(A).whp : arg = (i,MyP,s,e+1,r) ==> P res ] >= p.
+proof. progress. bypr.
+move => &m ae. 
+have zz : Pr[M(A).whp_if_end((i,MyP,s,e,r)) @ &m : P res] >= p.
+byphoare (_: arg = ((i,MyP,s,e,r)) ==> _).
+  conseq H.  progress.  auto.
+apply (lll Pr[M(A).whp_if_end(i, MyP, s, e, r) @ &m : P res] ). auto.
+byequiv.
+symmetry. conseq whp_split_if_end. smt(). auto. auto. auto. 
+qed.
+
+
+lemma asdsad (p : real) ia r MyPa: 
+   (phoare[ A.run : arg = ia ==> !MyPa res ] = p) =>
+  MyPa r = false => forall e, 0 <= e => 
+  phoare[ M(A).whp_if_end : arg = (ia, MyPa, 1,e,r) ==> !MyPa res ] = (p ^ (e+1)).
+proof. move => iipr ipr. apply ge0ind. smt().
+progress. simplify.
+  progress. proc.
+inline*. sp.
+rcondf 1. skip. smt().
+sp. 
+rcondt 1. skip. progress. smt().
+swap 1 1.  
+have f : phoare[ A.run : arg = ia ==> ! MyPa res] = (p^1). 
+simplify.  conseq iipr. smt(@Real).
+ call f. sp. skip. auto.
+  simplify.
+progress. proc.
+  have phf: phoare[ M(A).whp : arg = (ia, MyPa, 1, n+1, r) ==> !MyPa res] = (p ^(n+1)).
+ apply (whp_split_if_end'  MyPa ia 1 n r  (p^(n+1)) (fun x => !MyPa x) (H0 H) ).
+seq 1 : (!MyPa ri) (p ^(n+1)) p 1%r 0%r (i =  ia /\ MyP = MyPa /\ (!MyPa ri => M.c <= e + 1)).
+inline*. sp.
+seq 1 :  (i =  ia /\ MyP = MyPa /\ (!MyPa r0 => M.c <= e + 1)).
+ while (i = ia /\ i = i0 /\ MyP = MyP0 /\ MyP = MyPa /\ e = e0 /\ (!MyPa r0 => M.c <= e0 + 1)).
+wp. 
+call (_:true).  skip. progress. smt(). skip. progress. smt(). sp.  skip. progress. 
+ call phf. skip.  auto.
+rcondt 1. skip. progress. smt().  
+wp. simplify.  call iipr.  simplify.
+skip. progress. 
+hoare. 
+rcondf 1. skip.  progress. smt().
+simplify. skip. auto. smt(@Real).
+qed.
+
+lemma asdsad_le (p : real) ia r MyPa:
+   (phoare[ A.run : arg = ia ==> !MyPa res ] <= p) =>
+  MyPa r = false => forall e, 0 <= e =>
+  phoare[ M(A).whp_if_end : arg = (ia, MyPa, 1,e,r) ==> !MyPa res ] <= (p ^ (e+1)).
+proof. move => iipr ipr. apply ge0ind. smt().
+progress. simplify.
+  progress. proc.
+inline*. sp.
+rcondf 1. skip. smt().
+sp.
+rcondt 1. skip. progress. smt().
+swap 1 1.
+have f : phoare[ A.run : arg = ia ==> ! MyPa res] <= (p^1).
+conseq iipr. smt(@Real).
+call f. sp. skip. auto.
+  simplify.
+progress. proc.
+  have phf: phoare[ M(A).whp : arg = (ia, MyPa, 1, n+1, r) ==> !MyPa res] <= (p ^(n+1)).
+ apply (whp_split_if_end_le MyPa  ia 1 n r (p^(n+1))  (fun x => !MyPa x) (H0 H)  ).
+seq 1 : (!MyPa ri) (p ^(n+1)) p 1%r 0%r (i = ia /\ MyP = MyPa /\ (!MyPa ri => M.c <= e + 1)).
+inline*. sp.
+seq 1 :  (i = ia /\ MyP = MyPa /\ (!MyPa r0 => M.c <= e + 1)).
+ while (i = ia /\ i = i0 /\ MyP = MyP0 /\ MyP = MyPa /\ e = e0 /\ (!MyPa r0 => M.c <= e0 + 1)).
+wp.
+call (_:true).  skip. progress. smt(). skip. progress. smt(). sp.  skip. progress.
+ call phf. skip.  auto.
+rcondt 1. skip. progress. smt().
+wp. simplify.  call iipr.  simplify.
+skip. progress.
+hoare.
+rcondf 1. skip.  progress.  smt().
+simplify. skip. auto. smt(@Real).
+qed.
+
+lemma asdsad_ge (p : real) ia r MyPa:
+   (phoare[ A.run : arg = ia ==> !MyPa res ] >= p) =>
+  MyPa r = false => forall e, 0 <= e =>
+  phoare[ M(A).whp_if_end : arg = (ia, MyPa, 1,e,r) ==> !MyPa res ] >= (p ^ (e+1)).
+proof. move => iipr ipr. apply ge0ind. smt().
+progress. simplify.
+  progress. proc.
+inline*. sp.
+rcondf 1. skip. smt().
+sp.
+rcondt 1. skip. progress. smt().
+swap 1 1.
+have f : phoare[ A.run : arg = ia ==> ! MyPa res] >= (p^1).
+conseq iipr. smt(@Real).
+call f. sp. skip. auto.
+  simplify.
+progress. proc.
+  have phf: phoare[ M(A).whp : arg = (ia, MyPa, 1, n+1, r) ==> !MyPa res] >= (p ^(n+1)).
+ apply (whp_split_if_end_ge MyPa  ia 1 n r (p^(n+1))  (fun x => !MyPa x) (H0 H)  ).
+seq 1 : (!MyPa ri) (p ^(n+1)) p 1%r 0%r (i = ia /\ MyP = MyPa /\ (!MyPa ri => M.c <= e + 1)).
+inline*. sp.
+seq 1 :  (i = ia /\ MyP = MyPa /\ (!MyPa r0 => M.c <= e + 1)).
+ while (i = ia /\ i = i0 /\ MyP = MyP0 /\ MyP = MyPa /\ e = e0 /\ (!MyPa r0 => M.c <= e0 + 1)).
+wp.
+call (_:true).  skip. progress. smt(). skip. progress. smt(). sp.  skip. progress.
+ call phf. skip.  auto.
+rcondt 1. skip. progress. smt().
+wp. simplify.  call iipr.  simplify.
+skip. progress.
+hoare.
+rcondf 1. skip.  progress. smt().
+simplify. skip. auto. smt(@Real).
+qed.
+
+
+
+
+lemma asdsadq (p : real) ia MyP r :  
+   (phoare[ A.run : arg = ia ==> !MyP res ] = p) =>
+  MyP r = false => forall e, 0 <= e =>
+  phoare[ M(A).whp : arg = (ia,MyP,1,e+1,r) ==> !MyP res ] = (p ^ (e+1)).
+move => H1 H e ep.
+have fact1  : phoare[ M(A).whp_if_end : arg = (ia,MyP,1,e,r) ==> !MyP res ] = (p ^ (e+1)).
+apply (asdsad  p ia r  MyP H1 H e ep). auto.
+conseq (whp_split_if_end' MyP ia 1 e r (p^(e+1)) (fun x => !MyP x) fact1).
+qed.
+
+
+lemma asdsadq_le (p : real) ia MyP r:  
+   (phoare[ A.run : arg = ia ==> !MyP res ] <= p) =>
+  MyP r = false => forall e, 0 <= e =>
+  phoare[ M(A).whp : arg = (ia, MyP,1,e+1,r) ==> !MyP res ] <= (p ^ (e+1)).
+move => H1 H e ep.
+have fact1  : phoare[ M(A).whp_if_end : arg = (ia,MyP,1,e,r) ==> !MyP res ] <= (p ^ (e+1)).
+apply (asdsad_le   p  ia r MyP H1 H e ep). auto.
+conseq (whp_split_if_end_le MyP ia 1 e r (p^(e+1))  (fun x => !MyP x) fact1).
+qed.
+
+
+
+lemma asdsadq_ge (p : real) ia MyP r:  
+   (phoare[ A.run : arg = ia ==> !MyP res ] >= p) =>
+  MyP r = false => forall e, 0 <= e =>
+  phoare[ M(A).whp : arg = (ia, MyP,1,e+1,r) ==> !MyP res ] >= (p ^ (e+1)).
+move => H1 H e ep.
+have fact1  : phoare[ M(A).whp_if_end : arg = (ia,MyP,1,e,r) ==> !MyP res ] >= (p ^ (e+1)).
+apply (asdsad_ge   p  ia r MyP H1 H e ep). auto.
+conseq (whp_split_if_end_ge MyP ia 1 e r (p^(e+1))  (fun x => !MyP x) fact1).
+qed.
+
+
+
+end section.
+
+end IterUntilSucc.
+
+
+
